variables names, need to leave the linter on

src/Init/Data/Array/Basic.lean
@@ -1108,13 +1108,13 @@ We do not currently intend to provide verification theorems for these functions.
 Pads `l : Array α` on the left with repeated occurrences of `a : α` until it is of size `n`.
 If `l` is initially larger than `n`, just return `l`.
 -/
-def leftpad (n : Nat) (a : α) (l : Array α) : Array α := mkArray (n - l.size) a ++ l
+def leftpad (n : Nat) (a : α) (xs : Array α) : Array α := mkArray (n - xs.size) a ++ xs
 
 /--
 Pads `l : Array α` on the right with repeated occurrences of `a : α` until it is of size `n`.
 If `l` is initially larger than `n`, just return `l`.
 -/
-def rightpad (n : Nat) (a : α) (l : Array α) : Array α := l ++ mkArray (n - l.size) a
+def rightpad (n : Nat) (a : α) (xs : Array α) : Array α := xs ++ mkArray (n - xs.size) a
 
 /- ### reduceOption -/
 
